src/cbor/pulse/CBOR.Pulse.API.Borrow.Array.fsti
@@ -1,0 +1,30 @@
+module CBOR.Pulse.API.Borrow.Array
+open Pulse
+open CBOR.Pulse.API.Borrow
+open Pulse.Lib.Trade
+module A = Pulse.Lib.Array
+#lang-pulse
+
+inline_for_extraction
+val barray (a: lifetime) (t: Type0) : Type0
+
+val pts_to #a #t (r: barray a t) (v: Seq.seq t) : slprop
+
+unfold instance bref_pts_to #a #t : has_pts_to (barray a t) (Seq.seq t) = { pts_to = fun p #f r -> pts_to p r }
+
+instance val duplicable_pts_to #a #t (r: barray a t) v : duplicable (r |-> v)
+
+inline_for_extraction
+unobservable
+fn barray_of_array #a #t (r: A.array t) (#y: erased (Seq.seq t))
+  requires exists* p. a >:> A.pts_to r #p y
+  returns r: barray a t
+  ensures r |-> y
+
+inline_for_extraction
+unobservable
+fn use_bref #a #t (r: barray a t) (#y: erased (Seq.seq t))
+  requires a
+  requires r |-> y
+  returns r: A.array t
+  ensures exists* p. A.pts_to r #p y ** trade (A.pts_to r #p y) a
