src/cbor/pulse/CBOR.Pulse.API.Borrow.ArrayPtr.fsti
@@ -1,0 +1,40 @@
+module CBOR.Pulse.API.Borrow.ArrayPtr
+open Pulse
+open CBOR.Pulse.API.Borrow
+open Pulse.Lib.Trade
+module AP = Pulse.Lib.ArrayPtr
+open CBOR.Pulse.API.Borrow.Array
+#lang-pulse
+
+inline_for_extraction
+let bptr (a: lifetime) t = AP.ptr t
+
+let pts_to #a #t (r: bptr a t) (v: Seq.seq t) =
+  exists* p. a >:> AP.pts_to r #p v
+
+unfold instance bref_pts_to #a #t : has_pts_to (bptr a t) (Seq.seq t) = { pts_to = fun p #f r -> pts_to p r }
+
+instance val duplicable_pts_to #a #t (r: bptr a t) v : duplicable (r |-> v)
+
+inline_for_extraction
+unobservable
+fn bptr_of_ptr #a #t (r: AP.ptr t) (#y: erased (Seq.seq t))
+  requires exists* p. a >:> AP.pts_to r #p y
+  returns r: bptr a t
+  ensures r |-> y
+
+inline_for_extraction
+unobservable
+fn use_bref #a #t (r: bptr a t) (#y: erased (Seq.seq t))
+  requires a
+  requires r |-> y
+  returns r: AP.ptr t
+  ensures exists* p. AP.pts_to r #p y ** trade (AP.pts_to r #p y) a
+
+inline_for_extraction
+unobservable
+fn bptr_of_barray #a #t (r: barray a t) (len: SizeT.t) (#y: erased (Seq.seq t))
+  requires r |-> y
+  requires pure (Seq.length y == SizeT.v len)
+  returns r: bptr a t
+  ensures r |-> y
