src/cbor/pulse/CBOR.Pulse.API.Borrow.Ref.fst
@@ -1,0 +1,62 @@
+module CBOR.Pulse.API.Borrow.Ref
+open Pulse
+open CBOR.Pulse.API.Borrow
+open Pulse.Lib.Trade
+module R = Pulse.Lib.Reference
+#lang-pulse
+
+inline_for_extraction
+let bref (a: lifetime) t = ref t
+
+let pts_to #a #t (r: bref a t) (v: t) =
+  exists* p. a >:> R.pts_to r #p v
+
+fn dup_pts_to #a #t (r: bref a t) v () : duplicable_f (r |-> v) = {
+  unfold pts_to #a #t r v;
+  with p. assert a >:> R.pts_to r #p v;
+  dup (a >:> R.pts_to r #p v) ();
+  fold pts_to #a #t r v;
+  fold pts_to #a #t r v;
+}
+
+let duplicable_pts_to #a #t r v = { dup_f = dup_pts_to #a #t r v }
+
+inline_for_extraction
+fn read #a #t (r: bref a t) (#y: erased t)
+  preserves a
+  preserves r |-> y
+  returns x: t
+  ensures rewrites_to x (reveal y)
+{
+  unfold pts_to r y; with p. _;
+  dup (a >:> R.(pts_to r #p y)) ();
+  use_borrow a R.(pts_to r #p y);
+  let x = R.(!r);
+  elim_trade _ _;
+  fold pts_to r y;
+  x
+}
+
+inline_for_extraction
+unobservable
+fn bref_of_ref #a #t (r: ref t) (#y: erased t)
+  requires exists* p. a >:> R.pts_to r #p y
+  returns r: bref a t
+  ensures r |-> y
+{
+  fold pts_to #a #t r y;
+  r
+}
+
+inline_for_extraction
+unobservable
+fn use_bref #a #t (r: bref a t) (#y: erased t)
+  requires a
+  requires r |-> y
+  returns r: ref t
+  ensures exists* p. R.pts_to r #p y ** trade (R.pts_to r #p y) a
+{
+  unfold pts_to #a #t r y;
+  use_borrow a _;
+  r
+}
