src/cbor/pulse/CBOR.Pulse.API.Borrow.Ref.fsti
@@ -1,0 +1,35 @@
+module CBOR.Pulse.API.Borrow.Ref
+open Pulse
+open CBOR.Pulse.API.Borrow
+open Pulse.Lib.Trade
+#lang-pulse
+
+inline_for_extraction
+val bref (a: lifetime) (t: Type0) : Type0
+
+val pts_to #a #t (r: bref a t) (v: t) : slprop
+unfold instance bref_pts_to #a #t : has_pts_to (bref a t) t = { pts_to = fun p #f r -> pts_to p r }
+
+instance val duplicable_pts_to #a #t (r: bref a t) v : duplicable (r |-> v)
+
+inline_for_extraction
+fn read #a #t (r: bref a t) (#y: erased t)
+  preserves a
+  preserves r |-> y
+  returns x: t
+  ensures rewrites_to x (reveal y)
+
+inline_for_extraction
+unobservable
+fn bref_of_ref #a #t (r: ref t) (#y: erased t)
+  requires exists* p. a >:> r |-> Frac p y
+  returns r: bref a t
+  ensures a >:> r |-> y
+
+inline_for_extraction
+unobservable
+fn use_bref #a #t (r: bref a t) (#y: erased t)
+  requires a
+  requires r |-> y
+  returns r: ref t
+  ensures exists* p. r |-> Frac p y ** trade (r |-> Frac p y) a
