src/cbor/pulse/CBOR.Pulse.API.Borrow.Slice.fst
@@ -1,0 +1,48 @@
+module CBOR.Pulse.API.Borrow.Slice
+open Pulse
+open CBOR.Pulse.API.Borrow
+open Pulse.Lib.Trade
+module S = Pulse.Lib.Slice
+#lang-pulse
+
+inline_for_extraction
+let bslice (a: lifetime) t = S.slice t
+
+let pts_to #a #t (r: bslice a t) (v: Seq.seq t) =
+  exists* p. a >:> S.pts_to r #p v
+
+unfold instance bref_pts_to #a #t : has_pts_to (bslice a t) (Seq.seq t) = { pts_to = fun p #f r -> pts_to p r }
+
+fn dup_pts_to #a #t (r: bslice a t) v () : duplicable_f (r |-> v) = {
+  unfold pts_to #a #t r v;
+  with p. assert a >:> S.pts_to r #p v;
+  dup (a >:> S.pts_to r #p v) ();
+  fold pts_to #a #t r v;
+  fold pts_to #a #t r v;
+}
+
+let duplicable_pts_to #a #t r v = { dup_f = dup_pts_to #a #t r v }
+
+inline_for_extraction
+unobservable
+fn bslice_of_slice #a #t (r: S.slice t) (#y: erased (Seq.seq t))
+  requires exists* p. a >:> S.pts_to r #p y
+  returns r: bslice a t
+  ensures r |-> y
+{
+  fold pts_to #a #t r y;
+  r
+}
+
+inline_for_extraction
+unobservable
+fn use_bref #a #t (r: bslice a t) (#y: erased (Seq.seq t))
+  requires a
+  requires r |-> y
+  returns r: S.slice t
+  ensures exists* p. S.pts_to r #p y ** trade (S.pts_to r #p y) a
+{
+  unfold pts_to #a #t r y;
+  use_borrow a _;
+  r
+}
