src/cbor/pulse/CBOR.Pulse.API.Borrow.Slice.fsti
@@ -1,0 +1,62 @@
+module CBOR.Pulse.API.Borrow.Slice
+open Pulse
+open CBOR.Pulse.API.Borrow
+open Pulse.Lib.Trade
+module S = Pulse.Lib.Slice
+open CBOR.Pulse.API.Borrow.Array
+open CBOR.Pulse.API.Borrow.ArrayPtr
+#lang-pulse
+
+inline_for_extraction
+val bslice (a: lifetime) (t: Type0) : Type0
+
+inline_for_extraction
+val len #a #t (r: bslice a t) : SizeT.t
+
+val pts_to #a #t (r: bslice a t) (v: Seq.seq t) : slprop
+
+unfold instance bref_pts_to #a #t : has_pts_to (bslice a t) (Seq.seq t) = { pts_to = fun p #f r -> pts_to p r }
+
+instance val duplicable_pts_to #a #t (r: bslice a t) v : duplicable (r |-> v)
+
+ghost fn pts_to_len #a #t (r: bslice a t) (#y: erased (Seq.seq t))
+  preserves r |-> y
+  ensures pure (Seq.length y == SizeT.v (len r))
+
+inline_for_extraction
+unobservable
+fn bslice_of_slice #a #t (r: S.slice t) (#y: erased (Seq.seq t))
+  requires exists* p. a >:> S.pts_to r #p y
+  returns r: bslice a t
+  ensures r |-> y
+
+inline_for_extraction
+unobservable
+fn use_bref #a #t (r: bslice a t) (#y: erased (Seq.seq t))
+  requires a
+  requires r |-> y
+  returns r: S.slice t
+  ensures exists* p. S.pts_to r #p y ** trade (S.pts_to r #p y) a
+
+inline_for_extraction
+unobservable
+fn bslice_of_barray #a #t (r: barray a t) (len: SizeT.t) (#y: erased (Seq.seq t))
+  requires r |-> y
+  requires pure (Seq.length y == SizeT.v len)
+  returns r: bslice a t
+  ensures r |-> y
+
+inline_for_extraction
+unobservable
+fn bslice_of_bptr #a #t (r: bptr a t) (len: SizeT.t) (#y: erased (Seq.seq t))
+  requires r |-> y
+  requires pure (Seq.length y == SizeT.v len)
+  returns r: bslice a t
+  ensures r |-> y
+
+inline_for_extraction
+unobservable
+fn bptr_of_bslice #a #t (r: bslice a t) (#y: erased (Seq.seq t))
+  requires r |-> y
+  returns r: bptr a t
+  ensures r |-> y
