src/cbor/pulse/CBOR.Pulse.API.Borrow.fst
@@ -1,0 +1,79 @@
+module CBOR.Pulse.API.Borrow
+open Pulse
+open Pulse.Lib.Shift
+open Pulse.Lib.Trade
+module Trade = Pulse.Lib.Trade.Util
+module T = FStar.Tactics.V2
+#lang-pulse
+
+let (>:>) (a: lifetime) (p: slprop) : slprop =
+  shift a (p ** trade p a)
+
+instance duplicable_borrow a p : duplicable (a >:> p) = shift_duplicable _ _
+
+let borrowed ([@@@mkey] a: lifetime) (p: slprop) : slprop =
+  pure (a == p)
+
+fn dup_emp () : duplicable_f emp = {}
+instance duplicable_emp : duplicable emp = { dup_f = dup_emp }
+
+ghost fn borrow (p: slprop)
+  returns a: lifetime
+  ensures borrowed a p
+  ensures a >:> p
+{
+  fold borrowed p p;
+  intro (shift p (p ** trade p p)) fn _ { intro (trade p p) fn _ {} };
+  fold p >:> p;
+  p
+}
+
+ghost fn end_borrow (a: lifetime) (#p: slprop)
+  requires a
+  requires borrowed a p
+  ensures p
+{
+  unfold borrowed;
+  rewrite a as p;
+}
+
+ghost fn use_borrow (a: lifetime) (p: slprop)
+  requires a
+  requires a >:> p
+  ensures p
+  ensures trade p a
+{
+  unfold a >:> p;
+  elim_shift _ _;
+}
+
+ghost fn sub_borrow (a: lifetime) (p: slprop) (q: slprop)
+    (#[T.exact (`emp)] extra:slprop) {| duplicable extra |}
+    (f: unit -> stt_ghost unit emp_inames (p ** extra) (fun _ -> q ** trade q p))
+  requires a >:> p
+  requires extra
+  ensures a >:> q
+{
+  intro (shift a (q ** trade q a)) #(extra ** (a >:> p)) fn _ {
+    use_borrow a p;
+    f ();
+    Trade.trans q p a;
+  };
+  fold a >:> q;
+}
+
+inline_for_extraction
+fn with_borrow u#a (#t: Type u#a) (a: lifetime) (p: slprop) pre post
+    (f: unit -> stt t (p ** pre) (fun x -> p ** post x))
+  preserves a
+  preserves a >:> p
+  requires pre
+  returns x: t
+  ensures post x
+{
+  dup (a >:> p) ();
+  use_borrow a p;
+  let x = f ();
+  elim_trade _ _;
+  x
+}
