src/cbor/pulse/CBOR.Pulse.API.Borrow.fsti
@@ -1,0 +1,48 @@
+module CBOR.Pulse.API.Borrow
+open Pulse
+open Pulse.Lib.Trade
+module T = FStar.Tactics.V2
+#lang-pulse
+
+[@@erasable]
+type lifetime = slprop
+
+val (>:>) (a: lifetime) (p: slprop) : slprop
+
+instance val duplicable_borrow a p : duplicable (a >:> p)
+
+val borrowed ([@@@mkey] a: lifetime) (p: slprop) : slprop
+
+instance val duplicable_emp : duplicable emp
+
+ghost fn borrow (p: slprop)
+  returns a: lifetime
+  ensures borrowed a p
+  ensures a >:> p
+
+ghost fn end_borrow (a: lifetime) (#p: slprop)
+  requires a
+  requires borrowed a p
+  ensures p
+
+ghost fn use_borrow (a: lifetime) (p: slprop)
+  requires a
+  requires a >:> p
+  ensures p
+  ensures trade p a
+
+ghost fn sub_borrow (a: lifetime) (p: slprop) (q: slprop)
+    (#[T.exact (`emp)] extra:slprop) {| duplicable extra |}
+    (f: unit -> stt_ghost unit emp_inames (p ** extra) (fun _ -> q ** trade q p))
+  requires a >:> p
+  requires extra
+  ensures a >:> q
+
+inline_for_extraction
+fn with_borrow u#a (#t: Type u#a) (a: lifetime) (p: slprop) pre post
+    (f: unit -> stt t (p ** pre) (fun x -> p ** post x))
+  preserves a
+  preserves a >:> p
+  requires pre
+  returns x: t
+  ensures post x
