src/cddl/pulse/CDDL.Pulse.Bundle.ArrayGroup.fst
@@ -138,7 +138,7 @@ let array_bundle_set_parser_and_serializer
 inline_for_extraction noextract [@@noextract_to "krml"; bundle_get_impl_type_attr ]
 let bundle_array
   (#ty: Type0)
-  (#vmatch: perm -> ty -> cbor -> slprop)
+  (#vmatch: lifetime -> ty -> cbor -> slprop)
   (#cbor_array_iterator_t: Type)
   (#cbor_array_iterator_match: perm -> cbor_array_iterator_t -> list cbor -> slprop)
   (cbor_array_iterator_start: array_iterator_start_t vmatch cbor_array_iterator_match)
@@ -201,7 +201,7 @@ let bundle_array_group_ext'
 inline_for_extraction noextract [@@noextract_to "krml"; bundle_get_impl_type_attr]
 let bundle_array_group_item
   (#ty: Type0)
-  (#vmatch: perm -> ty -> cbor -> slprop)
+  (#vmatch: lifetime -> ty -> cbor -> slprop)
   (#cbor_array_iterator_t: Type)
   (#cbor_array_iterator_match: perm -> cbor_array_iterator_t -> list cbor -> slprop)
   (cbor_array_iterator_next: array_iterator_next_t vmatch cbor_array_iterator_match)
