src/cddl/pulse/CDDL.Pulse.Serialize.MapGroup.fsti
@@ -239,7 +239,7 @@ val impl_serialize_match_item_for
 
 inline_for_extraction noextract [@@noextract_to "krml"]
 val impl_serialize_map_zero_or_more
-  (#ty: Type0) (#vmatch: perm -> ty -> cbor -> slprop) (#cbor_map_iterator_t: Type0) (#cbor_map_iterator_match: perm -> cbor_map_iterator_t -> list (cbor & cbor) -> slprop)
+  (#ty: Type0) (#vmatch: lifetime -> ty -> cbor -> slprop) (#cbor_map_iterator_t: Type0) (#cbor_map_iterator_match: perm -> cbor_map_iterator_t -> list (cbor & cbor) -> slprop)
   (#ty2: Type0) (#vmatch2: perm -> ty2 -> (cbor & cbor) -> slprop)
   (map_share: share_t cbor_map_iterator_match)
   (map_gather: gather_t cbor_map_iterator_match)
